Updates.

LC/NV/UTLC/Sub/ReplaceFree.lean
@@ -8,25 +8,25 @@ open Term_
 
 
 /--
-  `replace_free u N M` := The simultaneous replacement of each occurrence of the variable `u` by the term `N` in the term `M`.
-  `M [ u := N ]`
-  (`u` -> `N` in `M`)
+  `replace_free v N M` := The simultaneous replacement of each occurrence of the variable `v` by the term `N` in the term `M`.
+  `M [ v := N ]`
+  (`v` -> `N` in `M`)
 -/
 def replace_free
-  (u : Symbol_)
+  (v : Symbol_)
   (N : Term_) :
   Term_ → Term_
   | var_ x =>
-    if u = x
+    if v = x
     then N
     else var_ x
 
-  | app_ P Q => app_ (replace_free u N P) (replace_free u N Q)
+  | app_ P Q => app_ (replace_free v N P) (replace_free v N Q)
 
   | abs_ x P =>
-    if u = x
+    if v = x
     then abs_ x P
-    else abs_ x (replace_free u N P)
+    else abs_ x (replace_free v N P)
 
 
 -------------------------------------------------------------------------------
@@ -34,23 +34,23 @@ def replace_free
 
 -- [1] lemma_1_2_5_iii_b
 lemma replace_free_id
-  (u : Symbol_)
-  (e : Term_) :
-  replace_free u (var_ u) e = e :=
+  (M : Term_)
+  (x : Symbol_) :
+  replace_free x (var_ x) M = M :=
   by
-    induction e
+    induction M
     all_goals
       unfold replace_free
-    case var_ x =>
+    case var_ x_ =>
       split_ifs
       case pos c1 =>
         rw [c1]
       case neg c1 =>
         rfl
-    case app_ P Q ih_1 ih_2 =>
+    case app_ P_ Q_ ih_1 ih_2 =>
       rw [ih_1]
       rw [ih_2]
-    case abs_ x P ih =>
+    case abs_ x_ P_ ih =>
       split_ifs
       case pos c1 =>
         rfl
@@ -60,111 +60,102 @@ lemma replace_free_id
 
 -- [1] lemma_1_2_5_i_b
 lemma replace_free_not_mem
-  (u : Symbol_)
-  (e1 : Term_)
-  (e2 : Term_)
-  (h1 : u ∉ e2.free_var_set) :
-  replace_free u e1 e2 = e2 :=
+  (M : Term_)
+  (x : Symbol_)
+  (N : Term_)
+  (h1 : x ∉ M.free_var_set) :
+  replace_free x N M = M :=
   by
-    induction e2
+    induction M
     all_goals
       unfold free_var_set at h1
       unfold replace_free
-    case var_ x =>
+    case var_ x_ =>
       simp at h1
 
       split_ifs
       rfl
-    case app_ P Q ih_1 ih_2 =>
+    case app_ P_ Q_ ih_1 ih_2 =>
       simp at h1
       obtain ⟨h1_left, h1_right⟩ := h1
 
       rw [ih_1 h1_left]
       rw [ih_2 h1_right]
-    case abs_ x P ih =>
+    case abs_ x_ P_ ih =>
       simp at h1
 
       split_ifs
       case pos c1 =>
         rfl
       case neg c1 =>
-        have s1 : u ∉ P.free_var_set := by tauto
+        have s1 : x ∉ P_.free_var_set := by tauto
         specialize ih s1
         rw [ih]
 
 
-lemma replace_free_inverse
-  (u v : Symbol_)
-  (e : Term_)
-  (h1 : v ∉ e.var_set) :
-  replace_free v (var_ u) (replace_free u (var_ v) e) = e :=
+lemma replace_free_mem_free_var_set
+  (M : Term_)
+  (x : Symbol_)
+  (N : Term_)
+  (y : Symbol_)
+  (h1 : y ∈ M.free_var_set)
+  (h2 : ¬ x = y) :
+  y ∈ (replace_free x N M).free_var_set :=
   by
-    induction e
-    all_goals
-      unfold var_set at h1
-      simp only [replace_free]
-    case var_ x =>
+    induction M
+    case var_ x_ =>
+      unfold free_var_set at h1
       simp at h1
+      rw [h1] at h2
 
+      unfold replace_free
       split_ifs
-      case pos c1 =>
-        rw [c1]
-        unfold replace_free
-        simp
-      case neg c1 =>
-        unfold replace_free
-        split_ifs
-        rfl
-    case app_ P Q ih_1 ih_2 =>
+      unfold free_var_set
+      simp
+      exact h1
+    case app_ P_ Q_ ih_1 ih_2 =>
+      unfold free_var_set at h1
       simp at h1
-      obtain ⟨h1_left, h1_right⟩ := h1
 
-      rw [ih_1 h1_left]
-      rw [ih_2 h1_right]
-    case abs_ x P ih =>
-      simp at h1
-      obtain ⟨h1_left, h1_right⟩ := h1
-      specialize ih h1_left
-
-      split_ifs
-      case pos c1 =>
-        unfold replace_free
-        split_ifs
-        congr
-        have s1 : v ∉ P.free_var_set :=
-        by
-          exact not_mem_var_set_imp_not_mem_free_var_set v P h1_left
-        exact replace_free_not_mem v (var_ u) P s1
-      case neg c1 =>
-        unfold replace_free
-        split_ifs
-        rw [ih]
-
-
-lemma replace_free_not_mem_free_var_set
-  (u v : Symbol_)
-  (e : Term_)
-  (h1 : ¬ u = v) :
-  u ∉ (replace_free u (var_ v) e).free_var_set :=
-  by
-    induction e
-    case var_ x =>
+      simp only [free_var_set]
+      simp
+      tauto
+    case abs_ x_ P_ ih =>
       unfold replace_free
       split_ifs
       case pos c1 =>
+        exact h1
+      case neg c1 =>
+        unfold free_var_set at h1
+        simp at h1
         unfold free_var_set
         simp
+        tauto
+
+
+lemma replace_free_not_mem_free_var_set
+  (M : Term_)
+  (x : Symbol_)
+  (N : Term_)
+  (h1 : x ∉ N.free_var_set) :
+  x ∉ (replace_free x N M).free_var_set :=
+  by
+    induction M
+    case var_ x_ =>
+      unfold replace_free
+      split_ifs
+      case pos c1 =>
         exact h1
       case neg c1 =>
         unfold free_var_set
         simp
         exact c1
-    case app_ P Q ih_1 ih_2 =>
+    case app_ P_ Q_ ih_1 ih_2 =>
       unfold replace_free
       unfold free_var_set
       simp
       exact ⟨ih_1, ih_2⟩
-    case abs_ x P ih =>
+    case abs_ x_ P_ ih =>
       unfold replace_free
       split_ifs
       case pos c1 =>
@@ -177,6 +168,54 @@ lemma replace_free_not_mem_free_var_set
         simp
         intro a1
         contradiction
+
+
+lemma replace_free_inverse
+  (M : Term_)
+  (x y : Symbol_)
+  (h1 : y ∉ M.var_set) :
+  replace_free y (var_ x) (replace_free x (var_ y) M) = M :=
+  by
+    induction M
+    all_goals
+      unfold var_set at h1
+      simp only [replace_free]
+    case var_ x_ =>
+      simp at h1
+
+      split_ifs
+      case pos c1 =>
+        rw [c1]
+        unfold replace_free
+        simp
+      case neg c1 =>
+        unfold replace_free
+        split_ifs
+        rfl
+    case app_ P_ Q_ ih_1 ih_2 =>
+      simp at h1
+      obtain ⟨h1_left, h1_right⟩ := h1
+
+      rw [ih_1 h1_left]
+      rw [ih_2 h1_right]
+    case abs_ x_ P_ ih =>
+      simp at h1
+      obtain ⟨h1_left, h1_right⟩ := h1
+      specialize ih h1_left
+
+      split_ifs
+      case pos c1 =>
+        unfold replace_free
+        split_ifs
+        congr
+        have s1 : y ∉ P_.free_var_set :=
+        by
+          exact not_mem_var_set_imp_not_mem_free_var_set y P_ h1_left
+        exact replace_free_not_mem P_ y (var_ x) s1
+      case neg c1 =>
+        unfold replace_free
+        split_ifs
+        rw [ih]
 
 
 #lint
